Split State into AbstractState and ConcreteState

Joinable.v
@@ -86,7 +86,7 @@ Global Instance pair_joinable : Joinable (prod A B) :=
 }.
 End pair_joinable.
 
-Section store_joinable.
+Section abstract_store_joinable.
 
 Lemma abstract_store_join_upperbound_left :
   forall s s', preorder s (abstract_store_join s s').
@@ -108,7 +108,7 @@ Global Instance abstract_store_joinable : Joinable abstract_store := {
   join_upper_bound_right := abstract_store_join_upperbound_right;
 }.
 
-End store_joinable.
+End abstract_store_joinable.
 
 Section unit_joinable.
 
@@ -136,3 +136,68 @@ Global Instance unit_joinable : Joinable unit :=
 
 End unit_joinable.
 
+Section nat_joinable.
+
+Lemma nat_max_upperbound_left :
+  forall n m, preorder n (Nat.max n m).
+Proof.
+  intros n m. revert n. induction m.
+  - destruct n; constructor.
+  - destruct n. 
+    + constructor. destruct m; auto with arith.
+    + simpl. apply le_n_S. apply IHm.
+Qed.
+
+Lemma nat_max_comm : 
+  forall n m, Nat.max n m = Nat.max m n.
+Proof.
+  intros n. induction n.
+  - destruct m; reflexivity.
+  - destruct m; simpl.
+    + reflexivity.
+    + rewrite IHn. reflexivity.
+Qed.
+    
+Lemma nat_max_upperbound_right :
+  forall n m, preorder m (Nat.max n m).
+Proof.
+  intros n m.
+  rewrite nat_max_comm. apply nat_max_upperbound_left.
+Qed.
+  
+Global Instance nat_joinable : Joinable nat :=
+{
+  join_op := Nat.max;
+  join_upper_bound_left := nat_max_upperbound_left;
+  join_upper_bound_right := nat_max_upperbound_right;
+}.
+
+End nat_joinable.
+
+Section store_joinable.
+
+Definition store_join (st1 st2 : store) : store :=
+  fun x => Nat.max (st1 x) (st2 x).
+
+Lemma store_join_upperbound_left :
+  forall st1 st2, preorder st1 (store_join st1 st2).
+Proof.
+  intros st1 st2. constructor. intro x.
+  simpl.  apply nat_max_upperbound_left.
+Qed.
+
+Lemma store_join_upperbound_right :
+  forall st1 st2, preorder st2 (store_join st1 st2).
+Proof.
+  intros st1 st2. constructor. intro x.
+  simpl. apply nat_max_upperbound_right.
+Qed.
+
+Global Instance store_joinable : Joinable store :=
+{
+  join_op := store_join;
+  join_upper_bound_left := store_join_upperbound_left;
+  join_upper_bound_right := store_join_upperbound_right;
+}.
+
+End store_joinable.
