Monad.v
@@ -1,3 +1,14 @@
+(*
+Inductive result
+  | return
+  | fail
+  | crashd
+in de monad state
+
+fix semantiek van catch mbv bovenstaande
+merge de evaluatie van bools en nats
+abstract en concrete values/monads/state/etc
+  *)
 Require Import Utf8.
 Require Import Coq.Classes.RelationClasses.
 
@@ -10,40 +21,6 @@ Inductive result (A : Type) : Type :=
   | returnR : A -> result A
   | crashed : result A
   | failed : result A.
-
-Definition State (S : Type) (A : Type) := 
-  S -> ((result A) * S)%type.
-
-Definition return_state (S A : Type) (x : A) : State S A :=
-  fun (st : S) => (returnR A x, st).
-
-Definition bind_state (S A B : Type) (m : State S A) (f : A -> State S B) 
-    : State S B :=
-  fun st => match m st with
-            | (returnR _ x, st') => f x st'
-            | (crashed _, st') => (crashed B, st')
-            | (failed _, st') => (failed B, st')
-            end.
-
-(*
-Inductive result
-  | return
-  | fail
-  | crashd
-in de monad state
-
-fix semantiek van catch mbv bovenstaande
-merge de evaluatie van bools en nats
-abstract en concrete values/monads/state/etc
-  *)
-
-Definition get {S : Type} : State S S := fun st => (returnR S st, st).
-
-Definition put {S : Type} (st' : S) : State S unit := 
-  fun st => (returnR unit tt, st').
-  
-Definition fail {S A : Type} : State S A :=
-  fun st => (failed A, st).
 
 Section result_preorder.
 Context {A : Type} `{PreorderedSet A}.
@@ -117,11 +94,56 @@ Global Instance result_joinable : Joinable (result A) := {
 
 End result_joinable.
 
+Definition State (A : Type) := 
+  store -> ((result A) * store)%type.
+
+Definition return_state (A : Type) (x : A) : State A :=
+  fun st => (returnR A x, st).
+
+Definition bind_state (A B : Type) (m : State A) (f : A -> State B) 
+    : State B :=
+  fun st => match m st with
+            | (returnR _ x, st') => f x st'
+            | (crashed _, st') => (crashed B, st')
+            | (failed _, st') => (failed B, st')
+            end.
+
+Definition get : State store := fun st => (returnR store st, st).
+
+Definition put (st' : store) : State unit := 
+  fun st => (returnR unit tt, st').
+  
+Definition fail {A : Type} : State A :=
+  fun st => (failed A, st).
+
+Definition AbstractState (A : Type) :=
+  abstract_store -> ((result A) * abstract_store)%type.
+
+Definition return_state_abstract (A : Type) (x : A) : AbstractState A :=
+  fun st => (returnR A x, st).
+
+Definition bind_state_abstract (A B : Type) 
+  (m : AbstractState A) (f : A -> AbstractState B) : AbstractState B :=
+  fun st => match m st with
+            | (returnR _ x, st') => f x st'
+            | (crashed _  , st') => (crashed B, st')
+            | (failed _   , st') => (failed B, st') 
+            end.
+
+Definition get_abstract : AbstractState abstract_store := 
+  fun st => (returnR abstract_store st, st).
+
+Definition put_abstract (st' : abstract_store) : AbstractState unit :=
+  fun st => (returnR unit tt, st').
+
+Definition fail_abstract {A : Type} : AbstractState A :=
+  fun st => (failed A, st).
+
 Section state_joinable.
-Context {S A : Type} `{Joinable S} `{Joinable A}.
+Context {A : Type}  `{Joinable A}.
 
 Definition join_state
-  (st1 st2 : State S A) : State S A :=
+  (st1 st2 : State A) : State A :=
   fun st => join_op (st1 st) (st2 st).
   
 Lemma join_state_upperbound_left : forall st st',
@@ -138,12 +160,42 @@ Proof.
   unfold join_state. simpl. apply pair_join_upperbound_right.
 Qed.
 
-Global Instance state_joinable : Joinable (State S A) := {
+Global Instance state_joinable : Joinable (State A) := {
   join_op := join_state;
   join_upper_bound_left := join_state_upperbound_left;
   join_upper_bound_right := join_state_upperbound_right;
 }.
 End state_joinable.
+
+Section abstract_state_joinable.
+Context {A : Type} `{Joinable A}.
+
+Definition join_state_abstract
+  (st1 st2 : AbstractState A) : AbstractState A :=
+  fun st => join_op (st1 st) (st2 st).
+
+Lemma join_state_abstract_upperbound_left : forall st st',
+  preorder st (join_state_abstract st st').
+Proof.
+  intros. simpl. constructor. intro x. simpl.
+  unfold join_state_abstract. apply pair_join_upperbound_left.
+Qed.
+
+Lemma join_state_abstract_upperbound_right : forall st st',
+  preorder st' (join_state_abstract st st').
+Proof.
+  intros. simpl. constructor. intro x. simpl.
+  unfold join_state_abstract. apply pair_join_upperbound_right.
+Qed.
+
+Global Instance abstract_state_joinable : Joinable (AbstractState A) := 
+{
+  join_op := join_state_abstract;
+  join_upper_bound_left := join_state_abstract_upperbound_left;
+  join_upper_bound_right := join_state_abstract_upperbound_right;
+}.
+
+End abstract_state_joinable.
 
 Class Monad (M : Type -> Type) : Type :=
 {
@@ -154,23 +206,39 @@ Arguments Build_Monad {_ _ _}.
 Arguments returnM {_ _ _}.
 Arguments bind {_ _ _ _}.
 
-Instance state_monad {S : Type} : Monad (State S) := {
-  returnM := (return_state S);
-  bind := (bind_state S);
+Instance state_monad : Monad (State) := {
+  returnM := (return_state);
+  bind := (bind_state);
+}.
+
+Instance abstract_state_monad : Monad (AbstractState) := {
+  returnM := return_state_abstract;
+  bind := bind_state_abstract;
 }.
 
 Section preordered_state.
-Context {S A : Type} `{PreorderedSet S, PreorderedSet A}.
+Context {A : Type} `{PreorderedSet A}.
 
 Lemma preorder_state : 
-  PreorderedSet (State S A).
+  PreorderedSet (State A).
 Proof. 
-  intros. unfold State. assert (PreorderedSet (A*S)). 
-  apply preorder_pairs. assert (PreorderedSet (option (A*S))).
+  intros. unfold State. assert (PreorderedSet (A*store)). 
+  apply preorder_pairs. assert (PreorderedSet (option (A*store))).
   apply preorder_option.
   apply preordered_function_spaces. 
 Qed.
 End preordered_state.
+
+Section preordered_abstract_state.
+Context {A : Type} `{PreorderedSet A}.
+
+Lemma preorder_abstract_state : PreorderedSet (AbstractState A).
+Proof.
+  intros. 
+  apply preordered_function_spaces.
+Qed.
+
+End preordered_abstract_state.
 
 Notation "x '<<' y ; z" := (bind y (fun x => z))
   (at level 20, y at level 100, z at level 200, only parsing).
