AbstractInterpreter.v
@@ -10,10 +10,15 @@ Require Import SharedInterpreter.
 
 Open Scope com_scope.
 
-Definition abstract_aexp := shared_aexp abstract_store parity 
-  extract_par parity_plus parity_mult.
+Definition abstract_aexp := shared_aexp 
+  parity 
+  extract_par 
+  parity_plus 
+  parity_mult
+  abstract_store
+  get_abstract.
 
-Fixpoint beval_abstract (b : bexp) : State abstract_store abstr_bool :=
+Fixpoint beval_abstract (b : bexp) : AbstractState abstr_bool :=
   match b with
   | BFalse => returnM (ab_false)
   | BTrue => returnM (ab_true)
@@ -34,37 +39,37 @@ Fixpoint beval_abstract (b : bexp) : State abstract_store abstr_bool :=
       returnM (and_ab b1' b2')
   end.
 
-Definition eval_if_abstract {S A} `{Joinable S, Joinable A} 
-  (b : abstr_bool) (st1 st2 : State S A) 
-  : State S A :=
+Definition eval_if_abstract {A} `{Joinable A} 
+  (b : abstr_bool) (st1 st2 : AbstractState A) 
+  : AbstractState A :=
   match b with
   | ab_true   => st1
   | ab_false  => st2
   | ab_top    => join_op st1 st2
-  | ab_bottom => fail
+  | ab_bottom => fail_abstract
   end.
   
-Definition eval_catch_abstract {S A} `{Joinable S, Joinable A} 
-  (st1 st2 : State S A) : State S A :=
+Definition eval_catch_abstract {A} `{Joinable A} 
+  (st1 st2 : AbstractState A) : AbstractState A :=
   fun st => match (st1 st) with
   | (crashed _, st') => (crashed A, st')
   | (failed _, st') => st2 st'
   | x => x
   end.
 
-Fixpoint ceval_abstract (c : com) : State abstract_store unit :=
+Fixpoint ceval_abstract (c : com) : AbstractState unit :=
   match c with
   | CSkip => returnM tt
   | c1 ;c; c2 =>
       (ceval_abstract c1) ;; (ceval_abstract c2)
   | x ::= a => 
       p << (abstract_aexp a) ;
-      st << get ;
-      put (t_update st x p)
+      st << get_abstract ;
+      put_abstract (t_update st x p)
   | CIf b c1 c2 => 
       b' << (beval_abstract b) ;
       eval_if_abstract b' (ceval_abstract c1) (ceval_abstract c2)
   | try c1 catch c2 => 
       eval_catch_abstract (ceval_abstract c1) (ceval_abstract c2)
-  | CFail => fail
+  | CFail => fail_abstract
   end.
