SharedInterpreter.v
@@ -1,22 +1,27 @@
 Require Import Language.
 Require Import Monad.
 
-Fixpoint shared_aexp (S V : Type)
+Fixpoint shared_aexp 
+  {state_type : Type -> Type} 
+  `{Monad state_type}
+  (V : Type)
   (extraction : nat -> V)
   (plus_op mult_op : V -> V -> V)
-  (e : aexp) :=
+  (store_type : Type)
+  (getter : state_type (string -> V))
+  (e : aexp) : state_type V :=
   match e with 
   | ANum n => returnM (extraction n)
   | AVar x =>
-      st << get ;
+      st << getter ;
       returnM (st x)
   | APlus e1 e2 =>
-      v1 << (shared_aexp S V extraction plus_op mult_op e1) ;
-      v2 << (shared_aexp S V extraction plus_op mult_op e2) ;
+      v1 << (shared_aexp V extraction plus_op mult_op store_type getter e1) ;
+      v2 << (shared_aexp V extraction plus_op mult_op store_type getter e2) ;
       returnM (plus_op v1 v2)
   | AMult e1 e2 =>
-      v1 << (shared_aexp S V extraction plus_op mult_op e1) ;
-      v2 << (shared_aexp S V extraction plus_op mult_op e2) ;
+      v1 << (shared_aexp V extraction plus_op mult_op store_type getter e1) ;
+      v2 << (shared_aexp V extraction plus_op mult_op store_type getter e2) ;
       returnM (mult_op v1 v2)
   end.
   
